\documentclass{article}
\usepackage{amsmath}

\begin{document}

$$\frac1{1} R_{1} \rightarrow R_{1}$$
$$R_{2} - (3) \cdot R_{1} \rightarrow R_{2}$$
$$\left[\begin{matrix}1 & 2\\0 & -2\end{matrix}\right]$$
$$\frac1{-2} R_{2} \rightarrow R_{2}$$
$$R_{1} - (2) \cdot R_{2} \rightarrow R_{1}$$
$$\left[\begin{matrix}1 & 0\\0 & 1\end{matrix}\right]$$
$$Pivot:(0, 1)$$

\end{document}$$\frac1{a} R_{1} \rightarrow R_{1}$$
$$\frac1{d} R_{2} \rightarrow R_{2}$$
$$R_{1} - (b/a) \cdot R_{2} \rightarrow R_{1}$$
$$\left[\begin{matrix}1 - \frac{b c}{a d} & 0\\\frac{c}{d} & 1\end{matrix}\right]$$
$$Pivot:(0, 1)$$
$$\frac1{1} R_{1} \rightarrow R_{1}$$
$$R_{2} - (3) \cdot R_{1} \rightarrow R_{2}$$
$$\left[\begin{matrix}1 & 2\\0 & -2\end{matrix}\right]$$
$$\frac1{-2} R_{2} \rightarrow R_{2}$$
$$R_{1} - (2) \cdot R_{2} \rightarrow R_{1}$$
$$\left[\begin{matrix}1 & 0\\0 & 1\end{matrix}\right]$$
$$Pivot:(0, 1)$$
$$\frac1{1} R_{1} \rightarrow R_{1}$$
$$R_{2} - (0) \cdot R_{1} \rightarrow R_{2}$$
$$\left[\begin{matrix}1 & 2 & 3\\0 & 2 & 3\\0 & 1 & 2\end{matrix}\right]$$
$$R_{3} - (0) \cdot R_{1} \rightarrow R_{3}$$
$$\left[\begin{matrix}1 & 2 & 3\\0 & 2 & 3\\0 & 1 & 2\end{matrix}\right]$$
$$\frac1{2} R_{2} \rightarrow R_{2}$$
$$R_{1} - (2) \cdot R_{2} \rightarrow R_{1}$$
$$\left[\begin{matrix}1 & 0 & 0\\0 & 1 & \frac{3}{2}\\0 & 1 & 2\end{matrix}\right]$$
$$R_{3} - (1) \cdot R_{2} \rightarrow R_{3}$$
$$\left[\begin{matrix}1 & 0 & 0\\0 & 1 & \frac{3}{2}\\0 & 0 & \frac{1}{2}\end{matrix}\right]$$
$$\frac1{1/2} R_{3} \rightarrow R_{3}$$
$$R_{1} - (0) \cdot R_{3} \rightarrow R_{1}$$
$$\left[\begin{matrix}1 & 0 & 0\\0 & 1 & \frac{3}{2}\\0 & 0 & 1\end{matrix}\right]$$
$$R_{2} - (3/2) \cdot R_{3} \rightarrow R_{2}$$
$$\left[\begin{matrix}1 & 0 & 0\\0 & 1 & 0\\0 & 0 & 1\end{matrix}\right]$$
$$Pivot:(0, 1, 2)$$
